coq/Extract.v
@@ -31,25 +31,25 @@ Extract Inductive Defns.TTAtom =>  "tTAtom" [
  "Ttat_shiftK"  "Ttat_substK"  "Ttat_shiftTy"  "Ttat_substTy" "Ttat_subste" "Ttat_shifte" ].
 
 
-Extract Inductive Defns.eTy =>  "eTy" [ "Typestar_nl_tcon"
-                                         "Typestar_nl_pi_intro"
-                                         "Typestar_nl_pi_elim"
-                                         "Typestar_nl_mtvar"
-                                         "Typestar_nl_tvar"
+Extract Inductive Defns.eTy =>  "eTy" [ "Ety_tcon"
+                                         "Ety_pi_intro"
+                                         "Ety_pi_elim"
+                                         "Ety_mtvar"
+                                         "Ety_tvar"
                                      ].
 
-Extract Inductive Defns.ete =>  "ete" [ "Termstar_nl_con"
-                                         "Termstar_nl_ix"
-                                         "Termstar_nl_pi_intro"
-                                         "Termstar_nl_pi_elim"
-                                         "Termstar_nl_mvar"
-                                         "Termstar_nl_tvar"
+Extract Inductive Defns.ete =>  "ete" [ "Ete_con"
+                                         "Ete_ix"
+                                         "Ete_pi_intro"
+                                         "Ete_pi_elim"
+                                         "Ete_mvar"
+                                         "Ete_tvar"
                                      ].
 
-Extract Inductive Defns.eK =>  "eK" [ "Kindstar_nl_type"
-                                       "Kindstar_nl_pi_intro"
-                                       "Kindstar_nl_mkvar"
-                                       "Kindstar_nl_tvar"
+Extract Inductive Defns.eK =>  "eK" [ "Ek_type"
+                                       "Ek_pi_intro"
+                                       "Ek_mkvar"
+                                       "Ek_tvar"
                                    ].
 
 Extract Inductive Defns.TTAtom => "ttAtom" [ (* atom in TT *)
